Formulate BlockPtr syncedmem rep
Since the indirect block tree fans out, such that each indrep_n_tree
application causes multiple internal applications, not just one, the rep
has to be stated in such a way that it can be assembled out of the reps
for the individual pieces, hence the exists and piff.

Start pushing the change in rep through indget, indread, and inclear.

src/BlockPtr.v
@@ -25,7 +25,9 @@ Require Import FSLayout.
 Require Import AsyncDisk.
 Require Import Rounding.
 Require Import Errno.
+Require Import DiskSet.
 
+Import SyncedMem.
 Import ListNotations.
 
 Set Implicit Arguments.
@@ -183,26 +185,32 @@ Module BlockPtr (BPtr : BlockPtrSig).
 
   (************** indirect blocks *)
 
-   Definition indrep_n_helper bxp ibn iblocks :=
+   Definition indrep_n_helper (Fs : @pred _ addr_eq_dec bool) bxp ibn iblocks :=
     (if (addr_eq_dec ibn 0)
-      then [[ iblocks = repeat $0 NIndirect ]]
-      else [[ BALLOCC.bn_valid bxp ibn ]] * IndRec.rep ibn iblocks
+      then [[ iblocks = repeat $0 NIndirect]] *
+           [[ Fs <=p=> emp ]]
+      else [[ BALLOCC.bn_valid bxp ibn ]] * IndRec.rep ibn iblocks *
+           [[ Fs <=p=> ibn |->? ]]
     )%pred.
 
   (* indlvl = 0 if ibn is the address of an indirect block,
      indlvl = 1 for doubly indirect, etc. *)
 
-  Fixpoint indrep_n_tree indlvl bxp ibn l :=
+  Fixpoint indrep_n_tree indlvl bxp Fs ibn l :=
     (match indlvl with
-    | 0 => indrep_n_helper bxp ibn l
-    | S indlvl' => let divisor := NIndirect ^ indlvl in
-                    exists iblocks, indrep_n_helper bxp ibn iblocks *
-                    exists l_part, [[ l = concat l_part ]] *
-                    listmatch (fun ibn' l' => indrep_n_tree indlvl' bxp (# ibn') l') iblocks l_part
+    | 0 => indrep_n_helper Fs bxp ibn l
+    | S indlvl' =>
+      exists iblocks Fs' lFs,
+        [[ length lFs = NIndirect ]] *
+        [[ Fs <=p=> Fs' * pred_fold_left lFs ]] *
+        indrep_n_helper Fs' bxp ibn iblocks *
+        exists l_part, [[ l = concat l_part ]] *
+        listmatch (fun ibn'_fs l' =>
+          indrep_n_tree indlvl' bxp (snd ibn'_fs) (# (fst ibn'_fs)) l') (combine iblocks lFs) l_part
     end)%pred.
 
-  Hint Extern 0 (okToUnify (indrep_n_helper _ _ _) (indrep_n_helper _ _ _)) => constructor : okToUnify.
-  Hint Extern 0 (okToUnify (indrep_n_tree _ _ _ _) (indrep_n_tree _ _ _ _ )) => constructor : okToUnify.
+  Hint Extern 0 (okToUnify (indrep_n_helper _ _ _ _) (indrep_n_helper _ _ _ _)) => constructor : okToUnify.
+  Hint Extern 0 (okToUnify (indrep_n_tree _ _ _ _ _) (indrep_n_tree _ _ _ _ _ )) => constructor : okToUnify.
   Local Hint Extern 0 (okToUnify (listmatch _ ?a _) (listmatch _ ?a _)) => constructor : okToUnify.
   Local Hint Extern 0 (okToUnify (listmatch _ _ ?b) (listmatch _ _ ?b)) => constructor : okToUnify.
 
@@ -290,15 +298,15 @@ Module BlockPtr (BPtr : BlockPtrSig).
 
   Local Hint Extern 1 (incl ?a ?b) => incl_solve.
 
-  Theorem indrep_n_helper_valid : forall bxp bn l,
-    bn <> 0 -> indrep_n_helper bxp bn l <=p=> [[ BALLOCC.bn_valid bxp bn ]] * IndRec.rep bn l.
+  Theorem indrep_n_helper_valid : forall bxp bn Fs l,
+    bn <> 0 -> indrep_n_helper Fs bxp bn l <=p=> [[ BALLOCC.bn_valid bxp bn ]] * IndRec.rep bn l * [[ Fs <=p=> bn |->? ]].
   Proof.
     intros. unfold indrep_n_helper. destruct bn; try omega. simpl.
     split; cancel.
   Qed.
 
-  Theorem indrep_n_tree_valid : forall indlvl bxp ir l,
-    ir <> 0 -> indrep_n_tree indlvl bxp ir l <=p=> indrep_n_tree indlvl bxp ir l * [[ BALLOCC.bn_valid bxp ir ]].
+  Theorem indrep_n_tree_valid : forall indlvl bxp Fs ir l,
+    ir <> 0 -> indrep_n_tree indlvl bxp Fs ir l <=p=> indrep_n_tree indlvl bxp Fs ir l * [[ BALLOCC.bn_valid bxp ir ]].
   Proof.
     destruct indlvl; intros; simpl.
     repeat rewrite indrep_n_helper_valid by auto. split; cancel.
@@ -307,14 +315,55 @@ Module BlockPtr (BPtr : BlockPtrSig).
     destruct_lifts. auto.
   Qed.
 
-  Lemma indrep_n_helper_0 : forall bxp l,
-    indrep_n_helper bxp 0 l <=p=> [[ l = repeat $0 NIndirect ]] * emp.
+  Lemma indrep_n_helper_0 : forall Fs bxp l,
+    indrep_n_helper Fs bxp 0 l <=p=> [[ l = repeat $0 NIndirect ]] * [[ Fs <=p=> emp ]].
   Proof.
     unfold indrep_n_helper; intros; split; cancel.
   Qed.
 
-  Theorem indrep_n_tree_0 : forall indlvl bxp l,
-    indrep_n_tree indlvl bxp 0 l <=p=> [[ l = repeat $0 (NIndirect ^ S indlvl)]].
+  Lemma pred_fold_left_Forall_emp: forall AT AEQ V (l : list (@pred AT AEQ V)),
+    Forall (fun x => x <=p=> emp) l ->
+    pred_fold_left l <=p=> emp.
+  Proof.
+    unfold pred_fold_left.
+    destruct l; auto; intros.
+    inversion H; subst.
+    clear H.
+    generalize dependent p.
+    induction l; cbn; intros.
+    auto.
+    inversion H3; subst.
+    apply IHl; auto.
+    rewrite H2.
+    rewrite H1.
+    split; cancel.
+  Qed.
+
+  Lemma pred_fold_left_cons: forall AT AEQ V (l : list (@pred AT AEQ V)) x,
+    pred_fold_left (x :: l) <=p=> x * pred_fold_left l.
+  Proof.
+    intros.
+    destruct l; cbn.
+    split; cancel.
+    generalize dependent p.
+    generalize dependent x.
+    induction l; cbn; intros.
+    split; cancel.
+    rewrite IHl.
+    rewrite IHl.
+    split; cancel.
+  Qed.
+
+  Lemma pred_fold_left_repeat_emp: forall AT AEQ V n,
+    pred_fold_left (repeat (@emp AT AEQ V) n) <=p=> emp.
+  Proof.
+    intros.
+    rewrite pred_fold_left_Forall_emp; auto.
+    auto using Forall_repeat.
+  Qed.
+
+  Theorem indrep_n_tree_0 : forall indlvl bxp Fs l,
+    indrep_n_tree indlvl bxp Fs 0 l <=p=> [[ l = repeat $0 (NIndirect ^ S indlvl)]] * [[ Fs <=p=> emp ]].
   Proof.
     induction indlvl; simpl; intros.
     rewrite mult_1_r, indrep_n_helper_0; split; cancel.
@@ -323,65 +372,115 @@ Module BlockPtr (BPtr : BlockPtrSig).
     destruct_lift H'.
     rewrite indrep_n_helper_0 in H.
     rewrite listmatch_length_pimpl in H; autorewrite with lists in *.
-    rewrite listmatch_lift_r with (F := fun x y => emp) in H.
+    destruct_lift H.
+    rewrite repeat_length, min_l in * by omega.
+    eapply listmatch_lift_r with (F := fun x y => ([[snd x <=p=> emp ]])%pred) in H.
+    rewrite listmatch_lift_l with (F := fun x y => emp) (P := fun x => snd x <=p=> emp) in H.
     rewrite listmatch_emp in H by cancel.
-    pred_apply; cancel.
+    destruct_lifts.
+    rewrite Forall_combine_r with (G := fun x => x <=p=> emp) in H2.
+    2: autorewrite with lists; congruence.
+    2: reflexivity.
+    rewrite pred_fold_left_Forall_emp in H4 by eauto.
+    (* working around a coq bug: "Conversion test raised an anomaly" when using 'pred_apply; cancel' *)
+    eapply sep_star_lift_apply'.
+    unfold lift_empty; intuition.
     erewrite concat_hom_repeat; eauto.
-    repeat f_equal. rewrite repeat_length in *. auto.
+    psubst.
+    split; cancel.
+    intros; split; cancel.
     intros; simpl.
-    destruct_lifts. erewrite repeat_spec with (y := x); eauto.
+    destruct_lifts.
+    destruct x.
+    eapply in_combine_l in H2 as ?.
+    erewrite repeat_spec with (y := w); eauto.
     rewrite IHindlvl. split; cancel.
-    cancel.
-    instantiate (iblocks := repeat $0 NIndirect).
-    instantiate (l_part := repeat (repeat $0 _) _).
+    norm. eassign Fs. cancel.
     rewrite indrep_n_helper_0.
-    rewrite listmatch_lift_r with (F := fun x y => emp) (P := fun y => length y = NIndirect ^ S indlvl).
+    cancel; eauto.
+    instantiate (l_part := repeat (repeat $0 _) _).
+    rewrite listmatch_lift_r with (F := fun x y => ([[ snd x <=p=> emp ]])%pred) (P := fun y => length y = NIndirect ^ S indlvl).
+    rewrite listmatch_lift_l with (F := fun x y => emp%pred) (P := fun y => snd y <=p=> emp).
     rewrite listmatch_emp_piff by auto.
     autorewrite with lists.
     cancel.
     apply Forall_repeat.
     autorewrite with lists. reflexivity.
-    intro x; intros.
-    erewrite repeat_spec with (y := x) by eauto.
+    rewrite Forall_combine_r with (G := fun x => x <=p=> emp).
+    apply Forall_repeat.
+    reflexivity.
+    repeat rewrite repeat_length; eauto.
+    reflexivity.
+    split; cancel.
+    intro x; destruct x; intros.
+    eapply in_combine_l in H.
+    erewrite repeat_spec with (y := w) by eauto.
     rewrite IHindlvl. split; cancel. subst. autorewrite with lists. auto.
     eapply repeat_spec; eauto.
-    subst.
+    intuition subst.
+    rewrite repeat_length; auto.
+    psubst.
+    rewrite pred_fold_left_Forall_emp.
+    split; cancel.
+    eapply Forall_repeat; auto.
     erewrite concat_hom_repeat; autorewrite with lists; auto.
+    rewrite min_l by omega.
+    eauto.
     apply Forall_repeat. auto.
   Qed.
 
-  Theorem indrep_n_helper_bxp_switch : forall bxp bxp' ir iblocks,
+  Lemma listmatch_indrep_n_tree_empty: forall indlvl bxp,
+    let iblocks := (repeat $0 NIndirect) in
+    indrep_n_helper emp bxp 0 iblocks *
+    listmatch (fun x y => indrep_n_tree indlvl bxp (snd x) # (fst x) y)
+      (combine iblocks (repeat emp NIndirect)) (repeat (repeat $0 (NIndirect ^ (S indlvl))) NIndirect) <=p=> emp.
+  Proof.
+    cbn -[Nat.div]; intros.
+    rewrite listmatch_emp_piff.
+    rewrite combine_length_eq; autorewrite with lists; eauto.
+    split; cancel.
+    intros.
+    rewrite combine_repeat in *.
+    eapply repeat_spec in H.
+    eapply repeat_spec in H0.
+    subst.
+    rewrite indrep_n_tree_0.
+    split; cancel.
+  Qed.
+
+  Theorem indrep_n_helper_bxp_switch : forall Fs bxp bxp' ir iblocks,
     BmapNBlocks bxp = BmapNBlocks bxp' ->
-    indrep_n_helper bxp ir iblocks <=p=> indrep_n_helper bxp' ir iblocks.
+    indrep_n_helper Fs bxp ir iblocks <=p=> indrep_n_helper Fs bxp' ir iblocks.
   Proof.
     intros. unfold indrep_n_helper, BALLOCC.bn_valid. rewrite H. reflexivity.
   Qed.
 
-  Theorem indrep_n_tree_bxp_switch : forall bxp bxp' indlvl ir l,
+  Theorem indrep_n_tree_bxp_switch : forall bxp bxp' indlvl Fs ir l,
     BmapNBlocks bxp = BmapNBlocks bxp' ->
-    indrep_n_tree indlvl bxp ir l <=p=> indrep_n_tree indlvl bxp' ir l.
+    indrep_n_tree indlvl bxp Fs ir l <=p=> indrep_n_tree indlvl bxp' Fs ir l.
   Proof.
     induction indlvl; intros; simpl.
-    apply indrep_n_helper_bxp_switch; auto.
-    split; cancel; rewrite indrep_n_helper_bxp_switch.
+    rewrite indrep_n_helper_bxp_switch by eassumption.
+    split; cancel.
+    split; cancel; eauto; rewrite indrep_n_helper_bxp_switch.
     all : try rewrite listmatch_piff_replace; try cancel; auto.
-    all : intros; simpl; rewrite IHindlvl; auto.
+    all : intros x; destruct x; intros; simpl; rewrite IHindlvl; auto.
   Qed.
 
-  Theorem listpred_indrep_n_tree_0 : forall indlvl bxp l,
-    listpred (fun l' => indrep_n_tree indlvl bxp 0 l') l <=p=>
-      [[ Forall (fun x => x = repeat $0 (NIndirect ^ S indlvl)) l ]].
+  Theorem listpred_indrep_n_tree_0 : forall indlvl bxp Fs l,
+    listpred (fun l' => indrep_n_tree indlvl bxp Fs 0 l') l <=p=>
+      [[ Forall (fun x => x = repeat $0 (NIndirect ^ S indlvl) /\ (Fs <=p=> emp))%type l ]].
   Proof.
     induction l; intros.
     - split; cancel. constructor.
     - simpl. rewrite IHl.
       rewrite indrep_n_tree_0.
       split; cancel.
-      all : match goal with [H : Forall _ _ |- _] => inversion H; auto end.
+      all : match goal with [H : Forall _ _ |- _] => inversion H; intuition end.
   Qed.
 
-  Lemma indrep_n_helper_length : forall bxp ibn l m,
-    indrep_n_helper bxp ibn l m -> length l = NIndirect.
+  Lemma indrep_n_helper_length : forall Fs bxp ibn l m,
+    indrep_n_helper Fs bxp ibn l m -> length l = NIndirect.
   Proof.
     unfold indrep_n_helper, IndRec.rep, IndRec.items_valid.
     intros; destruct addr_eq_dec; destruct_lift H; unfold lift_empty in *;
@@ -389,16 +488,16 @@ Module BlockPtr (BPtr : BlockPtrSig).
     unfold IndRec.Defs.item in *; simpl in *. omega.
   Qed.
 
-  Lemma indrep_n_helper_length_piff : forall bxp ibn l,
-    indrep_n_helper bxp ibn l <=p=> indrep_n_helper bxp ibn l * [[ length l = NIndirect ]].
+  Lemma indrep_n_helper_length_piff : forall Fs bxp ibn l,
+    indrep_n_helper Fs bxp ibn l <=p=> indrep_n_helper Fs bxp ibn l * [[ length l = NIndirect ]].
   Proof.
     intros.
     split; [> intros m H; apply indrep_n_helper_length in H as HH; pred_apply | ]; cancel.
   Qed.
 
-  Lemma indrep_n_length_pimpl : forall indlvl bxp ibn l,
-    indrep_n_tree indlvl bxp ibn l <=p=>
-    [[ length l = NIndirect ^ (S indlvl) ]] * indrep_n_tree indlvl bxp ibn l.
+  Lemma indrep_n_length_pimpl : forall indlvl bxp ibn Fs l,
+    indrep_n_tree indlvl bxp Fs ibn l <=p=>
+    [[ length l = NIndirect ^ (S indlvl) ]] * indrep_n_tree indlvl bxp Fs ibn l.
   Proof.
     induction indlvl; simpl; intros.
     intros; split; intros m H; destruct_lift H; pred_apply; cancel.
@@ -407,32 +506,40 @@ Module BlockPtr (BPtr : BlockPtrSig).
     rewrite indrep_n_helper_length_piff, listmatch_length_pimpl in H; destruct_lift H.
     rewrite listmatch_lift_r in H; destruct_lift H.
     erewrite concat_hom_length; eauto.
+    rewrite combine_length_eq in * by congruence.
+    eassign (NIndirect ^ S indlvl).
     f_equal; omega.
-    intros x y.
-    split; [> rewrite IHindlvl |]; cancel.
+    intros x y; destruct x.
+    intros.
+    rewrite IHindlvl.
+    instantiate (1 := fun x y => indrep_n_tree indlvl bxp (snd x) (# (fst x)) y).
+    split; cancel.
   Qed.
 
-  Lemma listmatch_indrep_n_tree_forall_length : forall indlvl bxp (l1 : list waddr) l2,
-    listmatch (fun ibn' l' =>indrep_n_tree indlvl bxp # (ibn') l') l1 l2 <=p=>
-    listmatch (fun ibn' l' =>indrep_n_tree indlvl bxp # (ibn') l') l1 l2 *
+  Lemma listmatch_indrep_n_tree_forall_length : forall indlvl bxp (l1 : list (waddr * _)) l2,
+    listmatch (fun a l' => indrep_n_tree indlvl bxp (snd a) # (fst a) l') l1 l2 <=p=>
+    listmatch (fun a l' => indrep_n_tree indlvl bxp (snd a) # (fst a) l') l1 l2 *
     [[Forall (fun sublist : list waddr => (length sublist = NIndirect * NIndirect ^ indlvl)%nat) l2]].
   Proof.
     intros.
     split; [> | cancel].
     rewrite listmatch_lift_r at 1. cancel. eauto.
-    intros. rewrite indrep_n_length_pimpl. split; cancel.
+    intros.
+    destruct x.
+    rewrite indrep_n_length_pimpl. split; cancel.
   Qed.
 
   Local Hint Extern 1 (Forall (fun x => length x = _) _) => match goal with
-    | [H : context [listmatch (fun x y => indrep_n_tree _ _ # x y) _ ?l]
+    | [H : context [listmatch (fun x y => indrep_n_tree _ (fst x) # (snd x) y) _ ?l]
         |- Forall (fun x => length x = _) ?l ] =>
           rewrite listmatch_indrep_n_tree_forall_length in H; destruct_lift H; solve [eassumption]
     | [|- Forall _ (upd_range ?l _ _ _)] => apply forall_upd_range; autorewrite with lists; eauto
   end.
 
-  Theorem indrep_n_helper_pts_piff : forall bxp ir l,
-    ir <> 0 -> indrep_n_helper bxp ir l <=p=> [[ length l = NIndirect ]] *
-                [[ BALLOCC.bn_valid bxp ir ]] * ir |-> (IndRec.Defs.block2val l, []).
+  Theorem indrep_n_helper_pts_piff : forall Fs bxp ir l,
+    ir <> 0 -> indrep_n_helper Fs bxp ir l <=p=> [[ length l = NIndirect ]] *
+                [[ BALLOCC.bn_valid bxp ir ]] * [[ Fs <=p=> ir |->? ]] *
+                ir |-> (IndRec.Defs.block2val l, []).
   Proof.
     intros.
     unfold indrep_n_helper, IndRec.rep. destruct addr_eq_dec; try omega.
@@ -443,51 +550,62 @@ Module BlockPtr (BPtr : BlockPtrSig).
     all : cancel.
   Qed.
 
-  Lemma indrep_n_tree_length: forall indlvl F ir l1 l2 bxp m, (F *
-    indrep_n_helper bxp ir l1 *
+  Lemma indrep_n_tree_length: forall indlvl F ir l1 l2 lfs bxp Fs m,
+    length lfs = NIndirect ->
+    (F *
+    indrep_n_helper Fs bxp ir l1 *
     listmatch
-     (fun ibn' l' => indrep_n_tree indlvl bxp # (ibn') l') l1 l2)%pred m->
+     (fun x l' => indrep_n_tree indlvl bxp (snd x) # (fst x) l') (combine l1 lfs) l2)%pred m->
      length (concat l2) = NIndirect * (NIndirect ^ (S indlvl)).
   Proof.
     intros.
-    rewrite indrep_n_helper_length_piff in H.
-    rewrite listmatch_length_pimpl in H.
-    erewrite listmatch_lift_r in H.
-    destruct_lift H.
+    rewrite indrep_n_helper_length_piff in H0.
+    rewrite listmatch_length_pimpl in H0.
+    erewrite listmatch_lift_r in H0.
+    destruct_lift H0.
+    rewrite combine_length_eq in * by congruence.
     erewrite concat_hom_length; eauto.
     f_equal; omega.
+
     intros.
+    destruct_lift H0.
+    instantiate (1 := fun x y => indrep_n_tree indlvl bxp (snd x) (# (fst x)) y).
     rewrite indrep_n_length_pimpl. split; cancel.
   Qed.
 
-  Lemma indrep_n_indlist_forall_length : forall F indlvl bxp ir l1 l2 m,
-    ((F ✶ indrep_n_helper bxp ir l1)
+  Lemma indrep_n_indlist_forall_length : forall F indlvl Fs bxp ir l1 fsl l2 m,
+    length fsl = NIndirect ->
+    ((F ✶ indrep_n_helper Fs bxp ir l1)
         ✶ listmatch
-            (fun ibn' l' =>indrep_n_tree indlvl bxp # (ibn') l') l1 l2)%pred m ->
+            (fun x l' => indrep_n_tree indlvl bxp (snd x) # (fst x) l') (combine l1 fsl) l2)%pred m ->
     Forall (fun sublist : list waddr => length sublist = NIndirect * NIndirect ^ indlvl) l2.
   Proof.
     intros.
-    rewrite indrep_n_helper_length_piff, listmatch_lift_r in H.
+    rewrite indrep_n_helper_length_piff, listmatch_lift_r in H0.
     destruct_lifts; eauto.
     intros x; intros.
-    rewrite indrep_n_length_pimpl. split; cancel.
+    rewrite indrep_n_length_pimpl.
+    split; cancel.
   Qed.
 
-  Lemma indrep_n_indlist_forall_length' : forall F F' indlvl bxp ir l1 l2 m,
-    (((F ✶ indrep_n_helper bxp ir l1)
+  Lemma indrep_n_indlist_forall_length' : forall F F' indlvl Fs bxp ir fsl l1 l2 m,
+    length fsl = NIndirect ->
+    (((F ✶ indrep_n_helper Fs bxp ir l1)
         ✶ listmatch
-            (fun ibn' l' =>indrep_n_tree indlvl bxp # (ibn') l') l1 l2) * F')%pred m ->
+            (fun x l' => indrep_n_tree indlvl bxp (snd x) # (fst x) l') (combine l1 fsl) l2) * F')%pred m ->
     Forall (fun sublist : list waddr => length sublist = NIndirect * NIndirect ^ indlvl) l2.
   Proof.
-    intros. eapply indrep_n_indlist_forall_length. eapply pimpl_apply; [> | exact H].
-    cancel.
+    intros. eapply indrep_n_indlist_forall_length.
+    2: eassign m; pred_apply; cancel.
+    auto.
   Qed.
 
-  Lemma indrep_index_bound_helper : forall Fm off indlvl bxp bn iblocks l_part m,
+  Lemma indrep_index_bound_helper : forall Fm Fs off indlvl bxp bn iblocks fsl l_part m,
       off < length (concat l_part) ->
-      ((Fm * indrep_n_helper bxp bn iblocks) *
-       listmatch (fun ibn' (l' : list waddr) =>
-                    indrep_n_tree indlvl bxp # (ibn') l') iblocks l_part)%pred m
+      length fsl = NIndirect ->
+      ((Fm * indrep_n_helper Fs bxp bn iblocks) *
+       listmatch (fun x l' =>
+                    indrep_n_tree indlvl bxp (snd x) # (fst x) l') (combine iblocks fsl) l_part)%pred m
       -> off / (NIndirect * NIndirect ^ indlvl) < NIndirect.
   Proof.
     intros.
@@ -496,17 +614,19 @@ Module BlockPtr (BPtr : BlockPtrSig).
     rewrite mult_comm; simpl in *. auto.
   Qed.
 
-  Lemma indrep_index_bound_helper' : forall Fm Fm' off indlvl bxp bn iblocks l_part m,
-    off < length (concat l_part) ->
-    ((Fm * indrep_n_helper bxp bn iblocks) *
-          listmatch (fun ibn' (l' : list waddr) =>
-            indrep_n_tree indlvl bxp # (ibn') l') iblocks l_part *
+  Lemma indrep_index_bound_helper' : forall Fm Fm' off indlvl bxp Fs bn iblocks l_part fsl m,
+      off < length (concat l_part) ->
+      length fsl = NIndirect ->
+    ((Fm * indrep_n_helper Fs bxp bn iblocks) *
+          listmatch (fun x (l' : list waddr) =>
+            indrep_n_tree indlvl bxp (snd x) # (fst x) l') (combine iblocks fsl) l_part *
             Fm')%pred m
     -> off / (NIndirect * NIndirect ^ indlvl) < NIndirect.
   Proof.
     intros.
     eapply indrep_index_bound_helper; eauto.
-    match goal with [H : _ |- _] => eapply pimpl_apply; [> | exact H]; cancel end.
+    eassign m.
+    pred_apply; cancel.
   Qed.
 
   Local Hint Resolve indrep_n_indlist_forall_length indrep_n_indlist_forall_length'.
@@ -597,9 +717,31 @@ Module BlockPtr (BPtr : BlockPtrSig).
     apply Nat.div_lt_upper_bound; auto.
     rewrite mult_comm. omega.
   Qed.
+  Lemma listmatch_combine_l_length: forall A B C AT AEQ V (prd : _ -> _ -> @pred AT AEQ V)
+    (a : list A) (b : list B) (c : list C),
+    length a = length b ->
+    listmatch prd (combine a b) c =p=> [[ length a = length c /\ length b = length c ]]
+      * listmatch prd (combine a b) c.
+  Proof.
+    intros.
+    rewrite listmatch_length_pimpl at 1.
+    rewrite combine_length.
+    substl (length a).
+    rewrite Nat.min_id.
+    cancel.
+  Qed.
 
-  Theorem xform_indrep_n_helper : forall bxp ir l,
-    crash_xform (indrep_n_helper bxp ir l) <=p=> indrep_n_helper bxp ir l.
+  Lemma in_combine_repeat_l : forall A B (a : A) n (b : list B) x,
+    In x (combine (repeat a n) b) ->
+    fst x = a.
+  Proof.
+    induction n; cbn; intuition.
+    destruct b; cbn in *; intuition eauto.
+    subst; auto.
+  Qed.
+
+  Theorem xform_indrep_n_helper : forall Fs bxp ir l,
+    crash_xform (indrep_n_helper Fs bxp ir l) <=p=> indrep_n_helper Fs bxp ir l.
   Proof.
     unfold indrep_n_helper. intros.
     destruct addr_eq_dec; xform_norm.
@@ -607,8 +749,8 @@ Module BlockPtr (BPtr : BlockPtrSig).
     - rewrite IndRec.xform_rep. auto.
   Qed.
 
-  Theorem xform_indrep_n_tree : forall xp indlvl ir l,
-    crash_xform (indrep_n_tree indlvl xp ir l) <=p=> indrep_n_tree indlvl xp ir l.
+  Theorem xform_indrep_n_tree : forall xp indlvl Fs ir l,
+    crash_xform (indrep_n_tree indlvl xp Fs ir l) <=p=> indrep_n_tree indlvl xp Fs ir l.
   Proof.
     induction indlvl; intros; simpl.
     + rewrite xform_indrep_n_helper. auto.
@@ -622,7 +764,8 @@ Module BlockPtr (BPtr : BlockPtrSig).
         xform_normr.
         rewrite xform_listmatch.
         rewrite listmatch_piff_replace. cancel.
-        intros. simpl. rewrite IHindlvl. auto.
+        intros. simpl. rewrite IHindlvl.
+        all: auto.
   Qed.
 
   Hint Rewrite Nat.mul_1_r.
@@ -639,21 +782,30 @@ Module BlockPtr (BPtr : BlockPtrSig).
     | [ |- ?a * ?b = ?b * ?c ] => rewrite mult_comm with (n := b) (m := c)
     | [ |- ?b * ?a = ?b * ?c ] => rewrite mult_comm with (n := b) (m := a)
     | [ H : ?a < ?b * ?c |- ?a < ?d * ?c] => assert (d = b); [ | congruence ]
-    | [ H : context [indrep_n_tree _ _ _ ?l] |- context [length ?l] ] =>
+    | [ H : context [indrep_n_tree _ _ _ _ ?l] |- context [length ?l] ] =>
       rewrite indrep_n_tree_length in H; destruct_lift H
+    | [ H : context [indrep_n_helper _ _ _ ?l] |- context [length ?l] ] =>
+      replace (length l) with NIndirect in * by (rewrite indrep_n_helper_length_piff in H; destruct_lift H; auto)
+    | [ H : context [indrep_n_helper _ _ _ ?l], H' : context [length ?l] |- _ ] =>
+      replace (length l) with NIndirect in * by (rewrite indrep_n_helper_length_piff in H; destruct_lift H; auto)
     | [ |- ?off / ?N < ?N' ] => apply Nat.div_lt_upper_bound; [ mult_nonzero |]
     | [ |- ?off < ?N * NIndirect] => rewrite mult_comm
-    | [ H : context [indrep_n_helper _ _ ?l] |- context [length ?l] ] =>
-      replace (length l) with NIndirect in * by (rewrite indrep_n_helper_length_piff in H; destruct_lift H; auto)
-    | [ H : context [indrep_n_helper _ _ ?l], H' : context [length ?l] |- _ ] =>
-      replace (length l) with NIndirect in * by (rewrite indrep_n_helper_length_piff in H; destruct_lift H; auto)
+    (* try to get an argument to indrep_n_tree or indrep_n_helper *)
+    | [ H : context [listmatch _ (combine ?a ?b) ?c], H' : context [length ?c] |- _ ] =>
+      replace (length c) with (length a) in * by (rewrite listmatch_combine_l_length in H; destruct_lift H; omega)
+    | [ H : context [listmatch _ (combine ?a ?b) ?c], H' : context [length ?c] |- _ ] =>
+      replace (length c) with (length b) in * by (rewrite listmatch_combine_l_length in H; destruct_lift H; omega)
+    | [ H : context [listmatch _ (combine ?a ?b) ?c] |- context [length ?c] ] =>
+      replace (length c) with (length a) in * by (rewrite listmatch_combine_l_length in H; destruct_lift H; omega)
+    | [ H : context [listmatch _ (combine ?a ?b) ?c] |- context [length ?c] ] =>
+      replace (length c) with (length b) in * by (rewrite listmatch_combine_l_length in H; destruct_lift H; omega)
     | [ H : context [listmatch _ ?a ?b] |- context [length ?b] ] =>
-      replace (length b) with (length a) in * by (rewrite listmatch_length_pimpl in H; destruct_lift H; auto)
-    | [ H : context [listmatch _ ?a ?b], H' : context [length ?b] |- _ ] =>
       replace (length b) with (length a) in * by (rewrite listmatch_length_pimpl in H; destruct_lift H; auto)
     | [ H : context [lift_empty _] |- _ ] => progress destruct_lift H
     | [ H : context [length (concat ?l)] |- _ ] => erewrite concat_hom_length in H by eauto
     | [ |- context [length (concat _)] ] => rewrite concat_hom_length by eauto
+    | [ |- context [Nat.min _ _] ] => rewrite min_l by omega
+    | [ H: context [Nat.min _ _] |- _ ] => rewrite min_l in H by omega
     | [ |- _ ] => omega
     end.
 
@@ -674,30 +826,68 @@ Module BlockPtr (BPtr : BlockPtrSig).
   end.
 
   Ltac indrep_n_tree_extract_lengths :=
-    repeat match goal with [H : context [indrep_n_tree _ _ _ ?x] |- _] =>
+    repeat match goal with [H : context [indrep_n_tree _ _ _ _ ?x] |- _] =>
       match goal with
       | [H' : length ?y = _ |- _] => tryif (unify x y) then fail 1 else fail
       | [|- _] => rewrite indrep_n_length_pimpl with (l := x) in H; destruct_lift H
       end
     end; try rewrite mult_1_r in *.
 
-  Theorem indrep_n_tree_repeat:
-    forall (indlvl : addr) (F : pred) (l1 : list waddr) (l2 : list (list waddr)) 
-      (bxp : balloc_xparams) (m : Mem.mem),
-    ((F ✶ indrep_n_helper bxp 0 l1)
-     ✶ listmatch (fun (ibn' : waddr) (l' : list waddr) => indrep_n_tree indlvl bxp # (ibn') l') l1 l2)%pred m ->
+  Ltac psubst :=
+    repeat match goal with p: pred |- _ =>
+      match goal with
+      | H: p <=p=> _ |- _ =>
+        rewrite H in *; clear H; clear p
+      | H: _ <=p=> p |- _ =>
+        rewrite <- H in *; clear H; clear p
+      end
+    end.
+
+  Theorem indrep_n_tree_repeat_concat:
+    forall indlvl F Fs lfs l1 l2 bxp m,
+    length lfs = NIndirect ->
+    ((F ✶ indrep_n_helper Fs bxp 0 l1)
+     ✶ listmatch (fun x y => indrep_n_tree indlvl bxp (snd x) # (fst x) y) (combine l1 lfs) l2)%pred m ->
     concat l2 = repeat $0 (NIndirect * NIndirect ^ S indlvl).
   Proof.
     intros. rewrite indrep_n_helper_0 in *. destruct_lifts.
     rewrite listmatch_length_pimpl in *; autorewrite with lists in *; destruct_lifts.
+    rewrite min_l in * by omega.
     erewrite concat_hom_repeat. repeat f_equal; auto.
     rewrite listmatch_lift_r in *. destruct_lifts; eauto.
-    intros. instantiate (1 := fun _ _ => emp). erewrite repeat_spec with (y := x); eauto.
+    intros. instantiate (1 := fun x y => ([[ snd x <=p=> emp ]])%pred).
+    erewrite in_combine_repeat_l by eauto.
     rewrite indrep_n_tree_0. split; cancel.
   Qed.
 
+  Theorem indrep_n_tree_repeat_Fs:
+    forall indlvl F Fs lfs l1 l2 bxp m,
+    length lfs = NIndirect ->
+    ((F ✶ indrep_n_helper Fs bxp 0 l1)
+     ✶ listmatch (fun x y => indrep_n_tree indlvl bxp (snd x) # (fst x) y) (combine l1 lfs) l2)%pred m ->
+    Fs * pred_fold_left lfs <=p=> emp.
+  Proof.
+    intros. rewrite indrep_n_helper_0 in *. destruct_lifts.
+    rewrite listmatch_lift_l in *.
+    destruct_lifts.
+    rewrite Forall_combine_r in *.
+    rewrite pred_fold_left_Forall_emp; eauto.
+    psubst; split; cancel.
+    autorewrite with lists; auto.
+    intros.
+    instantiate (1 := fun x => (snd x) <=p=> emp).
+    reflexivity.
+    intros.
+    erewrite in_combine_repeat_l by eauto.
+    rewrite roundTrip_0.
+    rewrite indrep_n_tree_0 at 1.
+    instantiate (1 := fun x y => ([[ y = _ ]])%pred).
+    split; cancel.
+  Qed.
+
+
   Hint Extern 1 (BALLOCC.bn_valid _ _) => match goal with
-    [H : context [indrep_n_helper _ ?ir] |- BALLOCC.bn_valid _ ?ir] =>
+    [H : context [indrep_n_helper _ _ ?ir] |- BALLOCC.bn_valid _ ?ir] =>
     rewrite indrep_n_helper_valid in H by omega; destruct_lift H; auto end.
 
   Local Hint Extern 1 (goodSize _ _) => match goal with
@@ -724,9 +914,9 @@ Module BlockPtr (BPtr : BlockPtrSig).
   Local Hint Resolve IndRec_items_valid_repeat IndRec.items_valid_updN IndRec.items_valid_upd_range.
   Local Hint Extern 1 (Rec.well_formed _) => unfold Rec.well_formed; cbn.
 
-  Lemma indrep_n_helper_items_valid : forall bxp bn l,
+  Lemma indrep_n_helper_items_valid : forall Fs bxp bn l,
     bn <> 0 ->
-    indrep_n_helper bxp bn l <=p=> [[ IndRec.items_valid bn l]] * indrep_n_helper bxp bn l.
+    indrep_n_helper Fs bxp bn l <=p=> [[ IndRec.items_valid bn l]] * indrep_n_helper Fs bxp bn l.
   Proof.
     intros.
     rewrite indrep_n_helper_length_piff.
@@ -735,7 +925,7 @@ Module BlockPtr (BPtr : BlockPtrSig).
   Qed.
 
   Local Hint Extern 1 (IndRec.items_valid _ _) => match goal with
-    [H : context [indrep_n_helper _ ?bn] |- IndRec.items_valid ?bn _] =>
+    [H : context [indrep_n_helper _ _ ?bn] |- IndRec.items_valid ?bn _] =>
     rewrite indrep_n_helper_items_valid in H; destruct_lift H end.
 
 
@@ -754,16 +944,16 @@ Module BlockPtr (BPtr : BlockPtrSig).
     }.
 
   Theorem indget_ok : forall indlvl lxp bxp bn off ms,
-    {< F Fm m0 m l,
+    {< F Fm Fs m0 sm m l,
     PRE:hm
-           LOG.rep lxp F (LOG.ActiveTxn m0 m) ms hm *
-           [[[ m ::: Fm * indrep_n_tree indlvl bxp bn l ]]] *
+           LOG.rep lxp F (LOG.ActiveTxn m0 m) ms sm hm *
+           [[[ m ::: Fm * indrep_n_tree indlvl Fs bxp bn l ]]] *
            [[ off < length l ]]
     POST:hm' RET:^(ms, r)
-           LOG.rep lxp F (LOG.ActiveTxn m0 m) ms hm' *
+           LOG.rep lxp F (LOG.ActiveTxn m0 m) ms sm hm' *
            [[ r = selN l off $0 ]]
     CRASH:hm'  exists ms',
-           LOG.rep lxp F (LOG.ActiveTxn m0 m) ms' hm'
+           LOG.rep lxp F (LOG.ActiveTxn m0 m) ms' sm hm'
     >} indget indlvl lxp bn off ms.
   Proof.
     induction indlvl; simpl.
@@ -772,13 +962,14 @@ Module BlockPtr (BPtr : BlockPtrSig).
       rewrite indrep_n_helper_valid by omega. cancel.
     + repeat safestep; autorewrite with core; try eassumption; clear IHindlvl.
       - erewrite indrep_n_tree_length in * by eauto.
-        erewrite indrep_n_tree_repeat; eauto.
+        erewrite indrep_n_tree_repeat_concat; eauto.
       - indrep_n_tree_bound.
       - rewrite indrep_n_helper_valid by omega.
         cancel.
-      - indrep_n_extract.
-        unfold IndRec.Defs.item; simpl. cancel.
-        all : indrep_n_tree_bound.
+      - rewrite listmatch_isolate with (i := off / (NIndirect ^ S indlvl))
+        by indrep_n_tree_bound.
+        rewrite selN_combine by indrep_n_tree_bound.
+        cbn [fst snd]; cancel.
       - match goal with [H : context [indrep_n_helper] |-_] => assert (HH := H) end.
         match goal with |- ?a mod ?n < ?b => replace b with n; auto end.
         rewrite listmatch_extract in HH; autorewrite with lists in *.
@@ -788,7 +979,8 @@ Module BlockPtr (BPtr : BlockPtrSig).
       - apply selN_selN_hom; eauto.
         indrep_n_tree_bound.
       Unshelve.
-      exact $0.
+      all: eauto.
+           exact ($0, emp).
   Qed.
 
   Local Hint Extern 1 ({{_}} Bind (indget _ _ _ _ _ ) _) => apply indget_ok : prog.
@@ -805,14 +997,14 @@ Module BlockPtr (BPtr : BlockPtrSig).
           let N := (NIndirect ^ (S indlvl')) in
           r <- ForEach b indbns' (rev indbns)
             Hashmap hm
-            Ghost [ F Fm iblocks l_part l bxp crash m0 m ]
+            Ghost [ F Fm Fs fsl iblocks l_part l bxp crash m0 sm m ]
             Loopvar [ ms r ]
             Invariant
               exists remlen, [[ remlen = length indbns' ]] *
-              LOG.rep lxp F (LOG.ActiveTxn m0 m) ms hm *
-              [[[ m ::: Fm * indrep_n_helper bxp ir iblocks *
-                        listmatch (fun ibn' l' => indrep_n_tree indlvl' bxp (# ibn') l')
-                          iblocks l_part ]]] *
+              LOG.rep lxp F (LOG.ActiveTxn m0 m) ms sm hm *
+              [[[ m ::: Fm * indrep_n_helper Fs bxp ir iblocks *
+                        listmatch (fun x l' => indrep_n_tree indlvl' bxp (snd x) (# (fst x)) l')
+                          (combine iblocks fsl) l_part ]]] *
               [[ r = skipn (remlen * (NIndirect ^ indlvl)) l ]]
             OnCrash crash
             Begin
@@ -824,15 +1016,15 @@ Module BlockPtr (BPtr : BlockPtrSig).
     }.
 
   Theorem indread_ok : forall indlvl lxp bxp ir ms,
-  {< F Fm m0 m l,
+  {< F Fm Fs m0 sm m l,
     PRE:hm
-           LOG.rep lxp F (LOG.ActiveTxn m0 m) ms hm *
-           [[[ m ::: Fm * indrep_n_tree indlvl bxp ir l ]]]
+           LOG.rep lxp F (LOG.ActiveTxn m0 m) ms sm hm *
+           [[[ m ::: Fm * indrep_n_tree indlvl Fs bxp ir l ]]]
     POST:hm' RET:^(ms, r)
-           LOG.rep lxp F (LOG.ActiveTxn m0 m) ms hm' *
+           LOG.rep lxp F (LOG.ActiveTxn m0 m) ms sm hm' *
            [[ r = l ]]
     CRASH:hm'  exists ms',
-           LOG.rep lxp F (LOG.ActiveTxn m0 m) ms' hm'
+           LOG.rep lxp F (LOG.ActiveTxn m0 m) ms' sm hm'
     >} indread indlvl lxp ir ms.
   Proof.
     induction indlvl; simpl.
@@ -843,7 +1035,7 @@ Module BlockPtr (BPtr : BlockPtrSig).
         destruct_lifts. unfold IndRec.Defs.item in *; simpl in *.
         rewrite firstn_oob by omega. auto.
     + hoare.
-      - erewrite indrep_n_tree_repeat; eauto. auto.
+      - erewrite indrep_n_tree_repeat_concat; eauto. auto.
       - rewrite indrep_n_helper_valid by omega. cancel.
       - rewrite firstn_oob by indrep_n_tree_bound.
         autorewrite with list.
@@ -853,11 +1045,14 @@ Module BlockPtr (BPtr : BlockPtrSig).
       - rewrite firstn_oob in * by indrep_n_tree_bound; subst.
         rewrite rev_eq_iff, rev_app_distr in *; cbn [rev] in *; subst.
         rewrite listmatch_extract.
+        rewrite selN_combine.
         rewrite selN_app1.
         rewrite selN_app2.
         rewrite sub_le_eq_0 by reflexivity; cbn [selN].
         cancel.
-        all : autorewrite with list; cbn; omega.
+        all: rewrite indrep_n_helper_length_piff in *; destruct_lifts.
+        all : autorewrite with list in *; cbn -[Nat.div] in *; try omega.
+        rewrite combine_length_eq; autorewrite with list; cbn; omega.
       - rewrite firstn_oob in * by indrep_n_tree_bound; subst.
         rewrite rev_eq_iff, rev_app_distr in *; cbn [rev] in *; subst.
         rewrite listmatch_length_pimpl in *; destruct_lifts.
@@ -866,8 +1061,11 @@ Module BlockPtr (BPtr : BlockPtrSig).
         rewrite <- (Nat.mul_1_l (NIndirect * NIndirect ^ indlvl)) at 1.
         rewrite <- Nat.mul_add_distr_r.
         repeat erewrite concat_hom_skipn by eauto.
-        erewrite skipn_selN_skipn with (off := length _) by omega.
+        erewrite skipn_selN_skipn with (off := length _).
         reflexivity.
+        rewrite combine_length_eq in H15.
+        autorewrite with list in *; cbn [length] in *; omega.
+        autorewrite with list; cbn [length]. omega.
       - apply LOG.rep_hashmap_subset; eauto.
     Grab Existential Variables.
       all : eauto; split.
@@ -886,20 +1084,22 @@ Module BlockPtr (BPtr : BlockPtrSig).
       | S indlvl' =>
         let^ (lms, indbns) <- IndRec.read lxp root 1 (BALLOCC.MSLog ms);
         let msn := BALLOCC.upd_memstate lms ms in
-        let^ (msn) <- ForN i < NIndirect
+        let^ (msn) <- ForEach bn indbns' indbns
           Hashmap hm
-          Ghost [ F Fm l_part bxp crash m0 freelist ]
+          Ghost [ F Fm Fs bxp crash m0 sm freelist l_part fsl ]
           Loopvar [ msn ]
           Invariant
-            exists m freelist' indbns' l_part', 
-            LOG.rep lxp F (LOG.ActiveTxn m0 m) (BALLOCC.MSLog msn) hm *
-            [[ l_part' = repeat (repeat $0 N) i ++ skipn i l_part ]] *
-            [[ indbns' = repeat $0 i ++ skipn i indbns ]] *
-            [[[ m ::: Fm * listmatch (fun ibn' l' => indrep_n_tree indlvl' bxp (# ibn') l') indbns' l_part'
-                         * BALLOCC.rep bxp freelist' msn ]]] * [[ incl freelist freelist' ]]
+            exists m freelist',
+            LOG.rep lxp F (LOG.ActiveTxn m0 m) (BALLOCC.MSLog msn) sm hm *
+            let n := length indbns - length indbns' in
+            [[[ m ::: Fm * listmatch (fun x l' => indrep_n_tree indlvl' bxp (snd x) (# (fst x)) l')
+                          (combine (skipn n indbns) (skipn n fsl)) (skipn n l_part)
+                         * BALLOCC.rep bxp freelist' msn ]]] *
+            [[ incl freelist freelist' ]] *
+            [[ (Fs * pred_fold_left (skipn n fsl) * BALLOCC.smrep freelist')%pred sm ]]
           OnCrash crash
           Begin
-            msn <- indclear_all indlvl' lxp bxp #(selN indbns i $0) msn;
+            msn <- indclear_all indlvl' lxp bxp # bn msn;
             Ret ^(msn)
           Rof ^(msn);
           Ret msn
@@ -907,54 +1107,119 @@ Module BlockPtr (BPtr : BlockPtrSig).
       BALLOCC.free lxp bxp root ms
     }.
 
+
   Theorem indclear_all_ok : forall indlvl lxp bxp ir ms,
     let N := NIndirect ^ indlvl in
-    {< F Fm m0 m l freelist,
+    {< F Fm Fs IFS m0 sm m l freelist,
     PRE:hm
-           LOG.rep lxp F (LOG.ActiveTxn m0 m) (BALLOCC.MSLog ms) hm *
-           [[[ m ::: (Fm * indrep_n_tree indlvl bxp ir l * 
-              BALLOCC.rep bxp freelist ms) ]]]
+           LOG.rep lxp F (LOG.ActiveTxn m0 m) (BALLOCC.MSLog ms) sm hm *
+           [[[ m ::: (Fm * indrep_n_tree indlvl bxp IFS ir l *
+              BALLOCC.rep bxp freelist ms) ]]] *
+           [[ (Fs * IFS * BALLOC.smrep freelist)%pred sm ]]
     POST:hm' RET: ms
-           exists m' freelist' l', 
-           LOG.rep lxp F (LOG.ActiveTxn m0 m') (BALLOCC.MSLog ms) hm' *
-           [[[ m' ::: (Fm * indrep_n_tree indlvl bxp 0 l' * 
+           exists m' freelist' l',
+           LOG.rep lxp F (LOG.ActiveTxn m0 m') (BALLOCC.MSLog ms) sm hm' *
+           [[[ m' ::: (Fm * indrep_n_tree indlvl bxp emp 0 l' *
               BALLOCC.rep bxp freelist' ms) ]]] *
+           [[ (Fs * BALLOC.smrep freelist')%pred sm ]] *
            [[ incl freelist freelist' ]]
-    CRASH:hm'  LOG.intact lxp F m0 hm'
+    CRASH:hm'  LOG.intact lxp F m0 sm hm'
     >} indclear_all indlvl lxp bxp ir ms.
     Proof.
-      unfold indclear_all.
       induction indlvl; simpl.
-      + hoare.
-        rewrite indrep_n_helper_pts_piff by auto.
-        rewrite indrep_n_helper_0. cancel.
-      + step. step.
+      + step.
+        hoare.
+        repeat rewrite indrep_n_helper_0. cancel.
+        rewrite indrep_n_helper_0 in *.
+        denote lift_empty as Hf; destruct_lift Hf.
+        psubst; auto.
+        destruct (addr_eq_dec ir 0). step.
+        rewrite indrep_n_helper_pts_piff in * by auto.
+        denote lift_empty as Hf; destruct_lift Hf.
+        psubst. denote exis as Hf; destruct_lift Hf.
+        hoare.
+        rewrite indrep_n_helper_0 by auto.
+        cancel.
+      + step.
+        psubst.
+        (* working around same "conversion anomaly" bug as above *)
+        prestep. norm. cancel.
+        rewrite indrep_n_tree_repeat_Fs with (m := list2nmem m) in *.
+        2: auto.
+        2: pred_apply; cancel.
+        intuition eauto.
+        pred_apply. cancel.
+        symmetry.
+        eapply indrep_n_tree_repeat_Fs with (m := list2nmem m); eauto.
+        pred_apply; cancel.
+        pred_apply; cancel.
+        auto.
         step.
         rewrite indrep_n_helper_valid by auto. cancel.
-        rewrite indrep_n_helper_length_piff in *. destruct_lifts.
+        rewrite indrep_n_helper_length_piff in *.
+        denote indrep_n_helper as Hi; destruct_lift Hi.
         unfold IndRec.Defs.item in *; simpl in *. rewrite firstn_oob by omega.
-        step.
-        - step.
-          rewrite listmatch_app_rev by (autorewrite with lists; auto).
-          rewrite listmatch_extract with (i := 0) (a := skipn _ _).
-          repeat rewrite skipn_selN, plus_0_r. cancel.
-          rewrite skipn_length. omega.
-          step.
-          rewrite indrep_n_tree_0. cancel.
-          unfold listmatch. simpl. rewrite indrep_n_tree_0. cancel.
-          rewrite combine_app by (autorewrite with lists; auto).
-          rewrite listpred_app. unfold removeN.
-          repeat rewrite skipn_skipn. cancel.
-          autorewrite with lists in *.
-          unfold removeN in *. repeat rewrite skipn_skipn in *. simpl in *. omega.
-        - step.
-          rewrite indrep_n_helper_pts_piff by auto. cancel.
-          step.
-          rewrite skipn_oob, app_nil_r by omega. rewrite indrep_n_helper_0.
+        prestep. norm. cancel.
+        rewrite Nat.sub_diag; cbn [skipn].
+        intuition auto.
+        - pred_apply; eassign dummy2. cancel.
+        - apply incl_refl.
+        - psubst.
+          pred_apply; cancel.
+          eassign ((Fs * dummy0)%pred). cancel.
+        - assert (length dummy2 = NIndirect) by indrep_n_tree_bound.
+          prestep. norml.
+          assert (length prefix < NIndirect).
+          rewrite indrep_n_helper_length_piff in *; destruct_lifts.
+          autorewrite with lists in *; cbn [length] in *; omega.
           cancel.
-        - eauto using LOG.intact_hashmap_subset.
+          autorewrite with lists; cbn [length].
+          repeat rewrite ?Nat.add_sub, ?Nat.sub_diag, ?skipn_app_r_ge by omega.
+          cbn [skipn].
+          erewrite skipn_selN_skipn by omega.
+          cbn [combine].
+          erewrite skipn_selN_skipn with (l := dummy2) by omega.
+          rewrite listmatch_cons.
+          cancel.
+          autorewrite with lists; cbn [length].
+          repeat rewrite Nat.add_sub.
+          erewrite skipn_selN_skipn with (l := dummy1) by omega.
+          rewrite pred_fold_left_cons.
+          cancel.
+          reflexivity.
+          step.
+          autorewrite with lists; cbn [length].
+          rewrite skipn_app_r_ge by omega.
+          repeat match goal with |- context [?b + S ?a - ?a] => replace (b + S a - a) with (S b) by omega end.
+          repeat match goal with |- context [S ?a - ?a] => replace (S a - a) with 1 by omega end.
+          rewrite indrep_n_tree_0. cancel.
+          autorewrite with lists; cbn [length].
+          repeat match goal with |- context [?b + S ?a - ?a] => replace (b + S a - a) with (S b) by omega end.
+          cancel.
+          cancel.
+        - rewrite indrep_n_helper_valid in * by auto.
+          denote lift_empty as Hl; destruct_lift Hl.
+          psubst.
+          denote piff as Hp. rewrite Hp in *.
+          prestep. norml.
+          repeat rewrite skipn_oob in * by omega.
+          rewrite Hp in *.
+          cancel.
+          rewrite skipn_oob by indrep_n_tree_bound.
+          rewrite indrep_n_helper_pts_piff by auto.
+          unfold listmatch; cancel.
+          safestep.
+          apply listmatch_indrep_n_tree_empty.
+          autorewrite with lists; auto.
+          rewrite pred_fold_left_repeat_emp.
+          split; cancel.
+          reflexivity.
+          cancel.
+        - cancel.
+          eauto using LOG.intact_hashmap_subset.
     Grab Existential Variables.
-    all : eauto; split.
+    all: try exact addr_eq_dec.
+    all : eauto using tt.
   Qed.
 
   Local Hint Extern 1 ({{_}} Bind (indclear_all _ _ _ _ _ ) _) => apply indclear_all_ok : prog.
@@ -1039,12 +1304,12 @@ Module BlockPtr (BPtr : BlockPtrSig).
            LOG.rep lxp F (LOG.ActiveTxn m0 m) (BALLOCC.MSLog ms) hm *
             [[ BALLOCC.bn_valid bxp ir ]] *
             [[ IndRec.items_valid ir indbns' ]] *
-           [[[ m ::: (Fm * indrep_n_helper bxp ir indbns) * 
+           [[[ m ::: (Fm * indrep_n_helper Fs bxp ir indbns) *
               BALLOCC.rep bxp freelist ms ]]]
     POST:hm' RET: ^(ms, ir')
            exists m' freelist', 
            LOG.rep lxp F (LOG.ActiveTxn m0 m') (BALLOCC.MSLog ms) hm' *
-           [[[ m' ::: (Fm * indrep_n_helper bxp ir' indbns' * 
+           [[[ m' ::: (Fm * indrep_n_helper Fs bxp ir' indbns' *
               BALLOCC.rep bxp freelist' ms) ]]] *
            [[ incl freelist freelist' ]] *
            ([[ ir' = 0 ]] \/ [[ ir' = ir ]])
@@ -1677,7 +1942,7 @@ Module BlockPtr (BPtr : BlockPtrSig).
            LOG.rep lxp F (LOG.ActiveTxn m0 m) ms hm * 
            [[ BALLOCC.bn_valid bxp ir ]] *
            [[ P -> ir = 0 ]] * [[ Q -> ir <> 0 ]] *
-           [[[ m ::: (Fm * indrep_n_helper bxp ir indbns) ]]]
+           [[[ m ::: (Fm * indrep_n_helper Fs bxp ir indbns) ]]]
     POST:hm' RET:^(ms, r)
            LOG.rep lxp F (LOG.ActiveTxn m0 m) ms hm' * 
            [[ r = indbns ]]
@@ -1737,12 +2002,12 @@ Module BlockPtr (BPtr : BlockPtrSig).
     PRE:hm
            LOG.rep lxp F (LOG.ActiveTxn m0 m) ms hm * 
            [[ BALLOCC.bn_valid bxp ir ]] *
-           [[[ m ::: (Fm * indrep_n_helper bxp ir indbns) ]]]
+           [[[ m ::: (Fm * indrep_n_helper Fs bxp ir indbns) ]]]
     POST:hm' RET: ms
            exists m' indbns', 
            LOG.rep lxp F (LOG.ActiveTxn m0 m') ms hm' *
            [[ indbns' = updN indbns to_grow ($ v) ]] *
-           [[[ m' ::: (Fm * indrep_n_helper bxp ir indbns') ]]]
+           [[[ m' ::: (Fm * indrep_n_helper Fs bxp ir indbns') ]]]
     CRASH:hm'  LOG.intact lxp F m0 hm'
     >} indput_upd_if_necessary lxp ir v indbns to_grow ms.
   Proof.
